Cpc/Proofs/Rules/Not_not_elim.lean
@@ -44,6 +44,9 @@ private theorem eo_interprets_of_not_false (M : SmtModel) (F : Term) :
       | Map _ =>
           exfalso
           simpa [hEvalF, __smtx_model_eval_not, SmtEval.native_not] using hEvalNot
+      | Fun _ =>
+          exfalso
+          simpa [hEvalF, __smtx_model_eval_not, SmtEval.native_not] using hEvalNot
       | Set _ =>
           exfalso
           simpa [hEvalF, __smtx_model_eval_not, SmtEval.native_not] using hEvalNot
@@ -51,6 +54,9 @@ private theorem eo_interprets_of_not_false (M : SmtModel) (F : Term) :
           exfalso
           simpa [hEvalF, __smtx_model_eval_not, SmtEval.native_not] using hEvalNot
       | Char _ =>
+          exfalso
+          simpa [hEvalF, __smtx_model_eval_not, SmtEval.native_not] using hEvalNot
+      | UValue _ _ =>
           exfalso
           simpa [hEvalF, __smtx_model_eval_not, SmtEval.native_not] using hEvalNot
       | RegLan _ =>
